\documentclass[]{article}
\usepackage{enumerate}% http://ctan.org/pkg/enumerate
\usepackage{amsmath}
%opening
\title{}
\author{}

\begin{document}

\maketitle

\begin{abstract}

\end{abstract}

\section{}


\begin{enumerate}[(i)]
\item		 \[ f(x) = x^2 \,\] %%%={{noprint|ˆt2x</math>}}}}
\item		 \[ f(x) = 2x + 2 \,\] %%%={{noprint|ˆt2</math>}}}}
\item		 \[ f(x) = \frac{1}{2}x^2 \,\] %%%={{noprint|ˆtx</math>}}}}
\item		 \[ f(x) = 2x^2 + 4x + 4 \,\] %%%={{noprint|ˆt4x+4</math>}}}}
\item		 \[ f(x) = \sqrt{x+2} \,\] %%%={{noprint|ˆt\frac{1}{2\sqrt{x+2}}</math>}}}}
\item		 \[ f(x) = \frac{1}{x} \,\] %%%={{noprint|ˆt-\frac{1}{x^2}</math>}}}}
\item		 \[ f(x) = \frac{3}{x+1} \,\] %%%={{noprint|ˆt\frac{-3}{(x+1)^2}</math>}}}}
\item		 \[ f(x) = \frac{1}{\sqrt{x+1}} \,\] %%%={{noprint|ˆt\frac{-1}{2(x+1)^{3/2}}</math>}}}}
\item		 \[ f(x) = \frac{x}{x+2} \,\] %%%={{noprint|ˆt\frac{2}{(x+2)^2}</math>}}}}
\item		 \[ f(x) = 2x^2 + 4\,\] %%%={{noprint|ˆtf'(x)=4x</math>}}}}
\item		 \[ f(x) = 3\sqrt[3]{x}\,</math> \]
\item		 \[ f(x) = 2x^5+8x^2+x-78\,\] %%%={{noprint|ˆtf'(x)=10x^4+16x+1</math>}}}}
\item		 \[ f(x) = 7x^7+8x^5+x^3+x^2-x\,\] %%%={{noprint|ˆtf'(x)=49x^6+40x^4+3x^2+2x-1</math>}}}}
\item		\[ f(x) = \frac{1}{x^2}+3x^\frac{1}{3}\,\] %%%={{noprint|ˆtf'(x)=\frac{-2}{x^3}+\frac{1}{\sqrt[3]{x^2}}</math>}}}}

\item		 \[ f(x) = 3x^{15} + \frac{1}{17}x^2 +\frac{2}{\sqrt{x}} \,\] %%%={{noprint|ˆtf'(x)=45x^{14}+\frac{2}{17}x-\frac{1}{x\sqrt{x}}</math>}}}}
\item		 \[ f(x) = \frac{3}{x^4} - \sqrt[4]{x} + x \,\] %%%={{noprint|ˆtf'(x)=\frac{-12}{x^5}-\frac{1}{4\sqrt[4]{x^3}}+1</math>}}}}
\item		 \[ f(x) = 6x^{1/3}-x^{0.4} +\frac{9}{x^2} \,\] %%%={{noprint|ˆtf'(x)=\frac{2}{\sqrt[3]{x^2}}-\frac{0.4}{x^{0.6}}-\frac{18}{x^3}</math>}}}}
\item		 \[ f(x) = \frac{1}{\sqrt[3]{x}} + \sqrt{x} \,\] %%%={{noprint|ˆtf'(x)=\frac{-1}{3x\sqrt[3]{x}}+\frac{1}{2\sqrt{x}}</math>}}}}
%%%===Product Rule===		
\item		 \[ f(x) = (x^4+4x+2)(2x+3) \,\] %%%={{noprint|ˆt10x^4+12x^3+16x+16</math>}}}}
\item		 \[ f(x) = (2x-1)(3x^2+2) \,\] %%%={{noprint|ˆt18x^2-6x+4</math>}}}}
\item		 \[ f(x) = (x^3-12x)(3x^2+2x) \,\] %%%={{noprint|ˆt15x^4+8x^3-108x^2-48x</math>}}}}
\item		 \[ f(x) = (2x^5-x)(3x+1) \,\] %%%={{noprint|ˆt36x^5+10x^4-6x-1</math>}}}}
\item		. \[ f(x) = (5x^2+3)(2x+7)\,\] %%%={{noprint|ˆt30x^2+70x+6</math>}}}}
\item		. \[ f(x) = 3x^2(5x^2+1)^4 \,\] %%%={{noprint|ˆt6x(25x^2+1)(5x^2+1)^3</math>}}}}
\item		. \[ f(x) = x^3(2x^2-x+4)^4 \,\] %%%={{noprint|ˆtx^2(2x^2-x+4)^3(22x^2-7x+12)</math>}}}}
\item		. \[ f(x) = 5x^2(x^3-x+1)^3 \,\] %%%={{noprint|ˆt5x(x^3-x+1)^2(11x^3-2x+1)</math>}}}}
\item		. \[ f(x) = (2-x)^6(5+2x)^4 \,\] %%%={{noprint|ˆt2(x-2)^5(2x+5)^3(10x+7)</math>}}}}
\item		\[ f(x) = \frac{2x+1}{x+5} \,\] %%%={{noprint|ˆtf'(x)=\frac{9}{(x+5)^2}</math>}}}}
\item		 \[ f(x) = \frac{3x^4+2x +2}{3x^2+1} \,\] %%%={{noprint|ˆtf'(x)=\frac{18x^5+12x^3-6x^2-12x+2}{(3x^2+1)^2}</math>}}}}
\item		 \[ f(x) = \frac{x^\frac{3}{2}+1}{x+2} \,\] %%%={{noprint|ˆtf'(x)=\frac{x\sqrt{x}+6\sqrt{x}-2}{2(x+2)^2}</math>}}}}
%% \item		ˆtd(u) = \frac{u^3+2}{u^3} \,\] %%%={{noprint|ˆtd'(u)=-\frac{6}{u^4}</math>}}}}
\item		\[ f(x) = \frac{x^2+x}{2x-1} \,\] %%%={{noprint|ˆtf'(x)=\frac{2x^2-2x-1}{(2x-1)^2}</math>}}}}
\item		 \[ f(x) = \frac{x+1}{2x^2+2x+3} \,\] %%%={{noprint|ˆtf'(x)=\frac{-2x^2-4x+1}{(2x^2+2x+3)^2}</math>}}}}
\item		 \[ f(x) = \frac{16x^4+2x^2}{x} \,\] %%%={{noprint|ˆtf'(x)=48x^2+2</math>}}}}
\item		\[ f(x) = (x+5)^2 \,\] %%%={{noprint|ˆtf'(x)=2(x+5)</math>}}}}
%% 32. ˆtg(x) = (x^3 - 2x + 5)^2 \,\] %%%={{noprint|ˆtg'(x)=2(x^{3}-2x+5)(3x^{2}-2)</math>}}}}		
\item 		 \[ f(x) = \sqrt{1-x^2} \,\] %%%={{noprint|ˆtf'(x)=-\frac{x}{\sqrt{1-x^{2}}}</math>}}}}
\item 		 \[ f(x) = \frac{(2x+4)^3}{4x^3+1} \,\] %%%={{noprint|ˆtf'(x)=\frac{6(4x^{3}+1)(2x+4)^{2}-(2x+4)^{3}(12x^{2})}{(4x^{3}+1)^{2}}</math>}}}}
\item 		 \[ f(x) = (2x+1)\sqrt{2x+2} \,\] %%%={{noprint|ˆtf'(x)=2\sqrt{2x+2}+\frac{2x+1}{\sqrt{2x+2}}</math>}}}}
\item 		 \[ f(x) = \frac{2x+1}{\sqrt{2x+2}} \,\] %%%={{noprint|ˆtf'(x)=\frac{2x+3}{(2x+2)^{3/2}}</math>}}}}
\item 		 \[ f(x) = \sqrt{2x^2+1}(3x^4+2x)^2 \,\] %%%={{noprint|ˆtf'(x)=\frac{2x(3x^{4}+2x)^{2}}{\sqrt{2x^{2}+1}}+\sqrt{2x^{2}+1}(2)(3x^{4}+2x)(12x^{3}+2)</math>}}}}
\item 		\[ f(x) = \frac{2x+3}{(x^4+4x+2)^2} \,\] 
\item \[f(x) = \frac{2x+3}{(x^4+4x+2)^2}\]

%% ===Trigonometric functions===		
\item  \[f(x) = 3e^x-4\cos (x) - \frac{1}{4}\ln x\,\]
\item \[f(x) = \sin(x)+\cos(x)\,\]

\end{enumerate}
\end{document}
