

	\section*{MA4702 -  Revision of Differentiations}
	

\Large
	\noindent Revision of Differentiation in advance of the "Curve Sketching" component of course. Please note that short questions on differentation should be expected for the second midterm
	\begin{multicols}{2}
		\begin{enumerate}
			\item	\qquad	 $ f(x) = x^2 \,$ %%%={{noprint|ˆt2x</math>}}}}
			\item	\qquad	 $ f(x) = 2x + 2 \,$ %%%={{noprint|ˆt2</math>}}}}
			\item	\qquad	 $ f(x) = \frac{1}{2}x^2 \,$ %%%={{noprint|ˆtx</math>}}}}
			\item	\qquad	 $ f(x) = 2x^2 + 4x + 4 \,$ %%%={{noprint|ˆt4x+4</math>}}}}
			\item	\qquad	 $ f(x) = \sqrt{x+2} \,$ %%%={{noprint|ˆt\frac{1}{2\sqrt{x+2}}</math>}}}}
			\item		 \[ f(x) = \frac{1}{x} \,\] %%%={{noprint|ˆt-\frac{1}{x^2}</math>}}}}
			\item		 \[ f(x) = \frac{3}{x+1} \,\] %%%={{noprint|ˆt\frac{-3}{(x+1)^2}</math>}}}}
			\item		 \[ f(x) = \frac{1}{\sqrt{x+1}} \,\] %%%={{noprint|ˆt\frac{-1}{2(x+1)^{3/2}}</math>}}}}
				\item		 \[ f(x) = \frac{x}{x+2} \,\] %%%={{noprint|ˆt\frac{2}{(x+2)^2}</math>}}}}
				\end{enumerate}
			\end{multicols}
			

\subsubsection*{Selected Solutions}
\begin{framed}	
	\Large
	\begin{multicols}{2}
		\begin{enumerate}
			\item	\qquad	 $ 2x$			\item	\qquad	 $2$
			\item	\qquad	 $ x$
			\item	\qquad	 $ 4x+4$ \\
			\item		 \[ \frac{1}{2\sqrt{x+2}}\]
			\item		 \[ -\frac{1}{x^2}\]
			\item		 \[ \frac{-3}{(x+1)^2}\]
			\item \[\frac{-1}{2(x+1)^{3/2}}\]
			\item		\[\frac{2}{(x+2)^2}\]
		\end{enumerate}
	\end{multicols}
\end{framed}
\newpage

				\begin{multicols}{2}
					\begin{enumerate}
						
						\item		 \[ f(x) = 2x^2 + 4\,\] %%%={{noprint|ˆtf'(x)=4x</math>}}}}
						\item		 \[ f(x) = 3\sqrt[3]{x}\, \]
						\item		 \[ f(x) = 2x^5+8x^2+x-78\,\] %%%={{noprint|ˆtf'(x)=10x^4+16x+1</math>}}}}
						\item		 \[ f(x) = 7x^7+8x^5+x^3+x^2-x\,\] %%%={{noprint|ˆtf'(x)=49x^6+40x^4+3x^2+2x-1</math>}}}}
						\item		\[ f(x) = \frac{1}{x^2}+3x^\frac{1}{3}\,\] %%%={{noprint|ˆtf'(x)=\frac{-2}{x^3}+\frac{1}{\sqrt[3]{x^2}}</math>}}}}
						
						\item		 \[ f(x) = 3x^{15} + \frac{1}{17}x^2 +\frac{2}{\sqrt{x}} \,\] %%%={{noprint|ˆtf'(x)=45x^{14}+\frac{2}{17}x-\frac{1}{x\sqrt{x}}</math>}}}}
						\item		 \[ f(x) = \frac{3}{x^4} - \sqrt[4]{x} + x \,\] %%%={{noprint|ˆtf'(x)=\frac{-12}{x^5}-\frac{1}{4\sqrt[4]{x^3}}+1</math>}}}}
						\item		 \[ f(x) = 6x^{1/3}-x^{0.4} +\frac{9}{x^2} \,\] %%%={{noprint|ˆtf'(x)=\frac{2}{\sqrt[3]{x^2}}-\frac{0.4}{x^{0.6}}-\frac{18}{x^3}</math>}}}}
						\item		 \[ f(x) = \frac{1}{\sqrt[3]{x}} + \sqrt{x} \,\] %%%={{noprint|ˆtf'(x)=\frac{-1}{3x\sqrt[3]{x}}+\frac{1}{2\sqrt{x}}</math>}}}}
					\end{enumerate}
				\end{multicols}
				\newpage
